src/spec/03-theorems/system.lean
@@ -4,19 +4,19 @@ import «02-abstract».«properties»
 namespace Abstract
 
 def Legal (tr : Trace) : Prop :=
-  ∀ t : Nat, (AbstractModel.Properties.catalogue.all fun l =>
+  ∀ t : Nat, (Abstract.Properties.catalogue.all fun l =>
     match l.property with
     | .state f => f (tr t).now (tr t).state
     | .trans f => f (tr t).now (tr t).state (tr (t+1)).state) = true
 
 theorem valid_implies_legal (mat : Bool) (tr : Trace)
-    (hv : Valid mat tr) (h0 : (tr 0).state = AbstractModel.ServerState.init) :
+    (hv : Valid mat tr) (h0 : (tr 0).state = Abstract.State.init) :
     Legal tr := sorry
 
-def oid (suffix : String) : ServerModel.Ident := { origin := "o", suffix }
+def oid (suffix : String) : Protocol.Ident := { origin := "o", suffix }
 
-def extType      : ServerModel.OType := .external
-def tgtType      : ServerModel.OType := .runnable "w1"
-def deadlineType : ServerModel.OType := .deadline
+def extType      : Protocol.OType := .external
+def tgtType      : Protocol.OType := .runnable "w1"
+def deadlineType : Protocol.OType := .deadline
 
 end Abstract
